progs/client_lemmas.v
@@ -755,10 +755,10 @@ Lemma tc_eval_id_i:
 Proof.
 intros.
 unfold tc_environ in H.
-destruct rho; apply environ_lemmas.typecheck_environ_sound in H.
+destruct rho. 
 destruct H as [? _].
 destruct (H i true t H0) as [v [? ?]].
-unfold eval_id. simpl. rewrite H1. simpl; auto.
+unfold eval_id. simpl in *. rewrite H1. simpl; auto.
 destruct H2. inv H2. auto.
 Qed.
 
