veric/environ_lemmas.v
@@ -7,24 +7,6 @@ Require Import veric.compcert_rmaps.
 Require Import veric.Clight_lemmas.
 Require Import veric.expr.
 
-(*Environment typechecking soundness statements*)
-
-Definition tc_te_denote (te: tenviron) (tc: PTree.t (type * bool)) :=
-forall id b ty , tc ! id = Some (ty,b) -> exists v, (Map.get te id = Some v /\ ((is_true (negb b)) \/ (typecheck_val v ty) = true)). 
-
-Definition tc_ve_denote (ve: venviron) (tc: PTree.t type) :=
-forall id ty, tc ! id = Some (ty) ->
-exists v, Map.get ve id = Some(v,ty).
-
-Definition tc_mode_denote (rho:environ) (Delta:tycontext)  :=
-forall id t, (glob_types Delta) ! id = Some t ->
-(ve_of rho) id = None \/ exists t,  (var_types Delta) ! id = Some t. 
-
-
-Definition tc_ge_denote (ge: genviron) (tc: PTree.t global_spec) :=
-forall id  t,  tc ! id = Some t -> 
-((exists b, exists i, 
-(ge id = Some (Vptr b i, globtype t) /\ typecheck_val (Vptr b i) (globtype t) = true))).
 
 Lemma eqb_type_eq: forall t1 t2, eqb_type t1 t2 = proj_sumbool (type_eq t1 t2).
 Proof.
@@ -34,7 +16,7 @@ apply eqb_type_true in H; subst; simpl; auto.
 rewrite proj_sumbool_is_true; auto.
 destruct (type_eq t1 t2); simpl; subst.
 rewrite eqb_type_refl in H; auto.
-auto.
+auto. 
 Qed.
 
 Lemma In_fst_split : forall A B i (l: list (A * B)), In i (fst (split l)) <-> exists b : B, In (i,b) l.  
@@ -48,184 +30,9 @@ clear IHl. destruct (split l). simpl. auto. destruct (split l). destruct a. simp
 right. apply IHl. eauto. 
 Qed.
 
-
-Lemma typecheck_mode_eqv : forall rho Delta,
-same_env rho Delta (all_var_ids Delta) = true <->
-tc_mode_denote rho Delta. 
-Proof.
-intros. split; intros. unfold all_var_ids in H.
-intro. intros.
-assert (In id  (fst (split (PTree.elements (glob_types Delta))))). 
-rewrite In_fst_split. exists t. apply PTree.elements_correct. auto. 
-
-induction (fst (split (PTree.elements (glob_types Delta)))). unfold same_env in *. 
-
-simpl in *. inv H1. 
-
-simpl in H. rewrite andb_true_iff in *. destruct H. 
-simpl in H1. destruct H1. subst. unfold same_mode in H. 
-remember ((var_types Delta) ! id). destruct o. eauto.
-remember ((glob_types Delta) ! id). destruct o. 
-remember (ve_of rho id). destruct o; try congruence. auto. congruence.
-destruct IHl; auto. 
-
-unfold tc_mode_denote in *. unfold all_var_ids in *. 
-assert (forall id, In id  (fst (split (PTree.elements (glob_types Delta)))) ->
-    exists t, ((glob_types Delta) ! id) = Some t).
-intros. rewrite In_fst_split in H0. destruct H0. 
-apply PTree.elements_complete in H0. eauto.
-
-induction  (fst (split (PTree.elements (glob_types Delta)))). 
-auto.  simpl in *. rewrite IHl; auto. rewrite andb_true_iff; intuition. 
-specialize (H0 a). destruct H0; auto. unfold same_mode.
-specialize (H _ _ H0). destruct H. rewrite H. rewrite H0. destruct ((var_types Delta) ! a).
-auto. auto. destruct H. rewrite H. auto. 
-Qed. 
-
-
-Lemma typecheck_ve_eqv : forall dv ve,
-typecheck_var_environ (PTree.elements dv) ve  = true <->
-tc_ve_denote ve dv.
-Proof.
-intros; split; intros.
-unfold tc_ve_denote. intros.   
-assert (In (id, ty) (PTree.elements dv)). apply PTree.elements_correct.
-auto.
-assert (forall t: type, In (id,t) (PTree.elements dv) -> dv ! id = Some t).
-intros. apply PTree.elements_complete. auto.
- induction (PTree.elements dv). 
-  inv H1. 
-  simpl in H. destruct a. simpl in *.
-    remember (Map.get ve p). destruct o. 
-       destruct p0.
-             remember (eqb_type t t0). destruct b0.
-             symmetry in Heqb0. apply eqb_type_true in Heqb0. subst.
-             destruct H1. inv H1. specialize (H2 ty). intuition; eauto.
-
-             apply IHl; eauto.
-
-             simpl in *; congruence.
-
-       simpl in *. congruence.
-
-
- 
-(*other way now...*)
-assert (forall t1 id, In (id,t1) (PTree.elements dv) -> dv ! id = Some t1).
-intros. apply PTree.elements_complete. auto.
-induction (PTree.elements dv).
-  auto.
-
-  simpl in *. destruct a. 
-    remember (Map.get ve p). destruct o. 
-      destruct p0.
-        simpl in *. unfold tc_ve_denote in H.
-
-        assert (forall (t1 : type) (id : positive),
-          (p, t) = (id, t1) \/ In (id, t1) l -> dv ! id = Some t1) by auto.
-        specialize (H0 t p). intuition. specialize (H _ _ H0).
-        destruct H.  rewrite H in Heqo.  inv Heqo.
-        rewrite eqb_type_refl. simpl. apply IHl. intros. apply H1. auto.
-
-      simpl. spec IHl. intros. apply H0. auto. unfold tc_ve_denote in H.
-          edestruct H. auto. congruence. Qed.
- 
-Lemma typecheck_ge_eqv : forall dv ge,
-typecheck_glob_environ (PTree.elements dv) ge = true <-> tc_ge_denote ge dv.
-Proof.
-intros.  
-
-split; intros. 
-  unfold tc_ge_denote. intros. 
-   assert (In (id,t)  (PTree.elements dv)). 
-        apply PTree.elements_correct. auto. 
-   assert (forall t: global_spec, In (id,t) (PTree.elements dv) -> dv ! id = Some t).
-    intros. apply PTree.elements_complete. auto. 
-   
-   induction (PTree.elements dv). 
-    inv H1. 
-    simpl in H1. destruct a. simpl in H. remember (ge p). destruct o; try congruence.
-    destruct p0. destruct v; try congruence. remember (eqb_type (globtype g) t0).
-    destruct b0; simpl in H; try congruence. 
-    symmetry in Heqb0. apply eqb_type_true in Heqb0. subst. 
-    assert (typecheck_glob_environ l ge = true).
-      simpl in H.  if_tac in H; try congruence. 
-    destruct H1.  
-      inv H1. rewrite <- Heqo. eexists;  eexists. split. auto. 
-      remember (globtype t). destruct t0; simpl in H; try congruence; auto. 
-    destruct IHl; auto. intros. apply H2. simpl; auto.
-    destruct H4. destruct H4. eauto. 
-
-   unfold tc_ge_denote in *. 
-   assert (forall t1 id, In (id,t1) (PTree.elements dv) -> dv ! id = Some t1).
-    intros. apply PTree.elements_complete. auto.
-   induction (PTree.elements dv). 
-     auto. 
-     
-     simpl. destruct a. rewrite IHl; auto. 
-     clear IHl. unfold Map.get in H. edestruct H.  apply H0. simpl. left.
-     auto. destruct H1 as [i [? ?]]. rewrite H1. rewrite eqb_type_refl.
-     simpl. destruct (globtype g); simpl in H2; try congruence; auto. 
-
-     intros; auto. 
-     apply H0; auto. simpl; auto. 
-Qed. 
-     
-    
-Lemma typecheck_te_eqv : forall t te, typecheck_temp_environ (PTree.elements t) te = true
-<-> tc_te_denote te t.
-Proof. intros.
-split. intros. unfold tc_te_denote. intros.
-assert (In (id, (ty,b)) (PTree.elements t)).
-apply PTree.elements_correct. auto.
-induction (PTree.elements t). simpl in *.
-
-destruct H1. 
-
-simpl in *. destruct a. destruct p0.
-remember (Map.get te p). destruct o; try solve [inv H].
-remember (typecheck_val v t0). destruct b0; 
-destruct b1; simpl in *; try congruence; 
-(destruct H1; [ inv H1 | ]; eauto).  
-
-intros. unfold tc_te_denote in *. 
-assert (forall t1 id, In (id,t1) (PTree.elements t) -> t ! id = Some t1).
-intros. apply PTree.elements_complete. auto.
-induction (PTree.elements t). auto.
-
-simpl in *. 
-assert (forall (t1 : type * bool) (id : positive),
-     In (id, t1) (a :: l) -> t ! id = Some t1) by auto.
-destruct a. destruct p0.
-specialize (H0 (t0, b) p). spec H0; auto.
-specialize (H p b t0). 
-destruct H. auto. 
-destruct H. rewrite H. destruct H2; rewrite H2. apply IHl. intros.
-simpl in H1. specialize (H1 t1 id). intuition. 
-destruct b; simpl in *; auto. 
-Qed.
-
-
-Lemma typecheck_environ_sound : forall ge te ve Delta,
-typecheck_environ (mkEnviron ge ve te) Delta = true ->
-tc_te_denote te (temp_types Delta) /\ tc_ve_denote ve (var_types Delta) /\ 
-tc_ge_denote ge (glob_types Delta).
-Proof.
-intros.
-unfold typecheck_environ in *. destruct Delta. destruct p.
-
-unfold temp_types in *. simpl in *. repeat rewrite andb_true_iff in *. intuition.
-destruct p. simpl in *. apply typecheck_te_eqv; auto.
-
-apply typecheck_ve_eqv; auto.
-
-apply typecheck_ge_eqv; auto.
-
-Qed.
-
-
 Lemma eqb_type_false: forall a b, eqb_type a b = false <-> a<>b.
-Admitted.
+Admitted. 
+
 
 Lemma join_te_denote : forall te1 te2 id b t1,
 (join_te te1 te2) ! id = Some (t1, b) ->
@@ -261,33 +68,18 @@ auto.
 auto.
 Qed. 
 
-Lemma same_env_ignores_t_ret : forall e0 e1 e2 e3 e4 e5 rho,
-same_env rho (e1,e2,e3,e4) (all_var_ids (e1,e2,e3,e4)) =
- same_env rho (e0,e2,e5,e4) (all_var_ids (e0,e2,e5,e4)).  
-intros. unfold all_var_ids. simpl. induction (fst (split (PTree.elements e4))). 
-auto. simpl. rewrite IHl.  auto. Qed.
-
-
-Lemma same_env_ignores_te : forall te te1 ve ge Delta,
-same_env (mkEnviron ge ve te) Delta (all_var_ids Delta) =
-same_env (mkEnviron ge ve te1) Delta (all_var_ids Delta). 
-intros. induction (all_var_ids Delta). auto.
-simpl. rewrite IHl. auto.
-Qed.
-
 Lemma typecheck_environ_join1:
   forall rho Delta1 Delta2, 
         var_types Delta1 = var_types Delta2 ->
         glob_types Delta1 = glob_types Delta2 ->
     
-        typecheck_environ rho Delta1 = true ->
-        typecheck_environ rho (join_tycon Delta1 Delta2) = true.
+        typecheck_environ Delta1 rho ->
+        typecheck_environ (join_tycon Delta1 Delta2) rho.
 Proof. intros.
- unfold typecheck_environ in *. repeat rewrite andb_true_iff in *.
-destruct H1 as [[[? ?] ?] ?]. repeat split. clear H2 H3 H4.  
+ unfold typecheck_environ in *. 
+destruct H1 as [? [? [? ?]]]. repeat split. clear H2 H3 H4.  
 destruct rho. simpl in *. 
-rewrite  typecheck_te_eqv in *.  
-unfold tc_te_denote in *. intros. unfold temp_types in *.
+unfold typecheck_temp_environ in *. intros. unfold temp_types in *.
 destruct Delta2. destruct p. destruct p. simpl in *. destruct Delta1.
 destruct p. destruct p. simpl in *. apply join_te_denote in H2.
 destruct H2. destruct H2. destruct H3.
@@ -301,7 +93,8 @@ unfold join_tycon. destruct Delta2. destruct p. destruct p. destruct Delta1.
 repeat destruct p. unfold glob_types in *; simpl in *; subst; auto. 
 
 unfold join_tycon. destruct Delta2. destruct p. destruct p. destruct Delta1.
-repeat destruct p. erewrite same_env_ignores_t_ret. eauto. 
+repeat destruct p. simpl in *. subst. unfold same_env in *. 
+simpl in *. intros. specialize (H4 id t3 H0). auto.  
 Qed. 
 
 
@@ -309,18 +102,17 @@ Lemma typecheck_environ_join2:
   forall rho Delta1 Delta2, 
         var_types Delta1 = var_types Delta2 ->
         glob_types Delta1 = glob_types Delta2 ->
-        typecheck_environ rho Delta2 = true ->
-        typecheck_environ rho (join_tycon Delta1 Delta2) = true.
+        typecheck_environ Delta2 rho ->
+        typecheck_environ (join_tycon Delta1 Delta2) rho.
 Proof.
 intros.
- unfold typecheck_environ in *. repeat rewrite andb_true_iff in *. intuition.
-destruct rho. simpl in *. 
-rewrite  typecheck_te_eqv in *. clear H4 H5. 
-unfold tc_te_denote in *. intros. unfold temp_types in *.
+ unfold typecheck_environ in *.  intuition.
+destruct rho. simpl in *.
+unfold typecheck_temp_environ in *. intros. unfold temp_types in *.
 destruct Delta2. destruct p. destruct p. simpl in *. destruct Delta1.
-destruct p. destruct p. simpl in *. apply join_te_denote in H1.
-destruct H1. destruct H1. destruct H4.
-edestruct H2; eauto.  destruct H5. destruct H6; destruct b; eauto. 
+destruct p. destruct p. simpl in *. apply join_te_denote in H4.
+destruct H4. destruct H4. destruct H6.
+edestruct H2; eauto.  destruct H7. destruct H8; destruct b; eauto. 
 unfold join_tycon. destruct Delta2. 
 destruct p. destruct p. destruct Delta1. destruct p. destruct p.
 unfold join_te. unfold var_types in *.  simpl in *. subst. auto. 
@@ -330,15 +122,16 @@ repeat destruct p. unfold glob_types in *; simpl in *; subst; auto.
 
 unfold join_tycon. destruct Delta2. destruct p. destruct p. destruct Delta1.
 repeat destruct p. unfold var_types in *. simpl in H. subst. unfold glob_types in *.
-simpl in *. subst.  erewrite same_env_ignores_t_ret. eauto.
-
+simpl in *. subst. 
+unfold same_env in *. 
+eapply H5; eauto. 
 Qed.
 
 
 
 Lemma typecheck_val_ptr_lemma:
    forall rho Delta id t a,
-   typecheck_environ rho Delta = true ->
+   typecheck_environ Delta rho ->
    denote_tc_assert (typecheck_expr Delta (Etempvar id (Tpointer t a))) rho ->
    (*(temp_types Delta) ! id =  Some (Tpointer t a, init) ->*) (*modified for init changes*)
    strict_bool_val (eval_id id rho) (Tpointer t a) = Some true ->
@@ -348,9 +141,9 @@ intros. unfold strict_bool_val in *. unfold typecheck_val.
 simpl in H0. if_tac in H0; simpl in *; intuition.
 remember ((temp_types Delta) ! id). destruct o; simpl in *; intuition.
 destruct p. simpl in *.  destruct t0; intuition. 
-unfold eval_id. destruct rho.  apply typecheck_environ_sound in H.
-destruct H as [? _]. unfold tc_te_denote in *.
-edestruct H; eauto. destruct H2.  simpl.  rewrite H2.
+unfold eval_id. destruct rho.  
+destruct H as [? _]. unfold typecheck_temp_environ in *.
+edestruct H; eauto. destruct H2.  simpl.  simpl in H2. rewrite H2.
 destruct H3.
 destruct b; simpl in *; try congruence.
 rewrite andb_if in H0. remember (eqb_type t t0). repeat (if_tac in H0; intuition). 
@@ -362,15 +155,15 @@ Qed.
 
 
 Lemma typecheck_environ_put_te : forall ge te ve Delta id v ,
-typecheck_environ (mkEnviron ge ve te) Delta = true ->
+typecheck_environ  Delta (mkEnviron ge ve te) ->
 (forall t , ((temp_types Delta) ! id = Some t ->
   (typecheck_val v (fst t)) = true)) ->
-typecheck_environ (mkEnviron ge ve (Map.set id v te)) Delta = true.
+typecheck_environ  Delta (mkEnviron ge ve (Map.set id v te)).
 Proof. 
-intros. unfold typecheck_environ in *. simpl in *. repeat rewrite andb_true_iff in *.
-intuition. clear H2 H3. destruct Delta. destruct p. 
+intros. unfold typecheck_environ in *. simpl in *. 
+intuition. clear H H2 H4. destruct Delta. destruct p. 
 destruct p. unfold temp_types in *; simpl in *.
-rewrite typecheck_te_eqv in *. unfold tc_te_denote in *.
+unfold typecheck_temp_environ. 
 intros. edestruct H1; eauto. destruct H2. rewrite Map.gsspec.
 if_tac. subst. exists v; intuition. specialize (H0 (ty,b)). 
 simpl in *. right. 
@@ -378,32 +171,31 @@ apply H0. auto.
 
 simpl in *. exists x. intuition.
 
-erewrite same_env_ignores_te. eauto. 
-
 
 Qed.
 
 
 Lemma typecheck_environ_put_te' : forall ge te ve Delta id v ,
-typecheck_environ (mkEnviron ge ve te) Delta = true ->
+typecheck_environ  Delta (mkEnviron ge ve te) ->
 (forall t , ((temp_types Delta) ! id = Some t ->
   (typecheck_val v (fst t)) = true)) ->
-typecheck_environ (mkEnviron ge ve (Map.set id v te)) (initialized id Delta) = true.
+typecheck_environ (initialized id Delta) (mkEnviron ge ve (Map.set id v te)).
 Proof.
 intros. 
-assert (typecheck_environ (mkEnviron ge ve (Map.set id v te)) Delta = true).
+assert (typecheck_environ Delta (mkEnviron ge ve (Map.set id v te))).
 apply typecheck_environ_put_te; auto.
 
-unfold typecheck_environ in *. simpl in *. repeat rewrite andb_true_iff in *. 
-destruct H as [[[? ?] ?] ?]. destruct H1 as [[[? ?] ?] ?]. 
-repeat split. 
-
+unfold typecheck_environ in *. simpl in *.
+intuition.  
 
 destruct Delta. destruct p. destruct p.  unfold initialized. unfold temp_types in *.
-clear H2 H3 H4 H5 H6 H7. simpl in *. 
-rewrite typecheck_te_eqv in *. unfold tc_te_denote in *. intros. remember (t1 ! id).
-destruct o; try congruence; auto. destruct p. simpl in *. rewrite PTree.gsspec in *.
-if_tac in H2. inv H2. edestruct H1; eauto. destruct H2. destruct H3; eauto. exists v.
+clear H1 H3 H4 H5 H8 H7. simpl in *. 
+unfold typecheck_temp_environ in *. 
+intros. remember (t1 ! id).
+destruct o; try congruence; auto. destruct p. simpl in *.
+rewrite PTree.gsspec in *.
+if_tac in H1. inv H1. 
+edestruct H; eauto. destruct H1. destruct H3; eauto. exists v.
 split. rewrite Map.gsspec in *. unfold ident_eq in *. rewrite peq_true in *. auto. 
 specialize (H0 (ty, b0)). right.  apply H0. auto. 
 eauto.
@@ -416,12 +208,11 @@ destruct p. simpl. unfold var_types. auto. auto.
 destruct Delta. destruct p. destruct p. simpl in *. unfold initialized.
 destruct ((temp_types (t1, t2, t0, t)) ! id); try destruct p; simpl in *; auto.
 
-erewrite same_env_ignores_te; eauto. unfold initialized.
-destruct Delta. simpl in *.  destruct p. destruct p. 
+unfold same_env in *. 
+intros. simpl in *. unfold initialized in *. 
+destruct Delta. simpl in *. destruct p. destruct p. 
 unfold var_types, temp_types in *. simpl in *. 
-destruct (t1 ! id); try destruct p;
-try erewrite same_env_ignores_t_ret;  eauto.
-
+destruct (t2 ! id); try destruct p; eauto. 
 Qed. 
 
 Lemma type_eq_true : forall a b, proj_sumbool  (type_eq a b) =true  -> a = b.
